
\documentclass[letterpaper,reqno,12pt]{article}
\usepackage[margin=1.0in]{geometry}
\usepackage{color,latexsym,amsmath,amssymb}
\usepackage{fancyhdr}
\usepackage{amsthm}
\usepackage[linesnumbered,lined,boxed,commentsnumbered,noend,noline]{algorithm2e}
\usepackage{dsfont}
\usepackage{graphicx}
\usepackage{hyperref}
\usepackage{lmodern}
\usepackage[numbers]{natbib}
\usepackage{listings}% http://ctan.org/pkg/listings
\lstset{
  basicstyle=\ttfamily,
  columns=fullflexible,
  mathescape
}

\setlength{\AlCapSkip}{0.5em}

\allowdisplaybreaks

\newcommand{\RR}{\mathbb{R}}
\newcommand{\CC}{\mathbb{C}}
\newcommand{\ZZ}{\mathbb{Z}}
\newcommand{\QQ}{\mathbb{Q}}
\newcommand{\NN}{\mathbb{N}}
\newcommand{\mynote}[3][red]
  {{\color{#1} \fbox{\bfseries\sffamily\scriptsize#2}
  {\small$\blacktriangleright$\textsf{\emph{#3}}$\blacktriangleleft$}}~}
\newcommand{\yp}[1]{\mynote{YP}{#1}}
\DeclareMathOperator{\conv}{conv}
\DeclareMathOperator{\charcone}{char.cone}
\DeclareMathOperator{\STAB}{STAB}
\DeclareMathOperator{\Down}{Down}
\DeclareMathOperator{\lca}{lca}
\DeclareMathOperator{\LPO}{LPO}
\DeclareMathOperator{\OPT}{OPT}
\DeclareMathOperator{\LHS}{LHS}
\DeclareMathOperator{\RHS}{RHS}
\DeclareMathOperator{\tr}{tr}
\DeclareMathOperator{\vol}{vol}
\DeclareMathOperator{\argmin}{arg\,min}
\DeclareMathOperator{\argmax}{arg\,max}
\DeclareMathOperator{\poly}{poly}
\begin{document}
\pagenumbering{arabic}
\title{Network Flow Algorithms: Exercise 1.4}
\author{Yuchong Pan}
\date{\today}
\newtheorem{theorem}{Theorem}
\newtheorem{lemma}{Lemma}
\newtheorem{claim}{Claim}
\theoremstyle{definition} \newtheorem{exercise}{Exercise} [section]
\theoremstyle{definition} \newtheorem{defn}{Definition}
\maketitle
%

We re-define $d_k(j)$ to be the length of the shortest $s$-$j$ path of length $k$, as in R.\ M.\ Karp's original paper \cite{karp1978characterization}.

Let $c' = c - \mu$. Let $\Gamma_0$ be a cycle of $G$. Then we have that
\begin{align*}
  c'\left(\Gamma_0\right) &= \sum_{e \in E\left(\Gamma_0\right)} c'(e) = \sum_{e \in E\left(\Gamma_0\right)} (c(e) - \mu) = \sum_{e \in E\left(\Gamma_0\right)} c(e) - \left|\Gamma_0\right| \mu = c\left(\Gamma_0\right) - \left|\Gamma_0\right| \min_{\text{cycle $\Gamma$ of $G$}} \frac{c(\Gamma)}{|\Gamma|} \\
  &\geq c\left(\Gamma_0\right) - \left|\Gamma_0\right| \cdot \frac{c\left(\Gamma_0\right)}{\left|\Gamma_0\right|} = c\left(\Gamma_0\right) - c\left(\Gamma_0\right) = 0.
\end{align*}
This shows that $G$ with edge costs $c'$ does not have negative-cost cycles. Hence, the Bellman-Ford algorithm correctly computes the shortest $s$-$j$ paths for all $j \in V$. Let $d_k'(j)$ be the length of the shortest $s$-$j$ path of length $k$ with edge costs $c'$. By Exercise 1.2, there exists a simple shortest path $P_j$ from $s$ to any $j \in V$, which is of length $< n$. Hence, $c'(P_j) = \min_{0 \leq k \leq n - 1} d_k'(j)$ and $c'(P_j) \leq d_n'(j)$ for all $j \in V$. This implies that $d_n'(j) \geq \min_{0 \leq k \leq n - 1} d_k'(j)$ for all $j \in V$. On the other hand, let $\Gamma^* = \argmin_{\text{cycle $\Gamma$ of $G$}} \frac{c(\Gamma)}{|G|}$. Then we have that
$$ c'\left(\Gamma^*\right) = c\left(\Gamma^*\right) - \left|\Gamma^*\right| \min_{\text{cycle $\Gamma$ of $G$}} \frac{c(\Gamma)}{|\Gamma|} = c\left(\Gamma^*\right) - \left|\Gamma^*\right| \cdot \frac{c\left(\Gamma^*\right)}{\left|\Gamma^*\right|} = c\left(\Gamma^*\right) - c\left(\Gamma^*\right) = 0. $$
Let $v \in V(\Gamma^*)$. Let $P$ be a simple shortest $s$-$v$ path. Then $|P| < n$. Let $\ell \in \NN$ be such that $|P| + \ell |\Gamma^*| \geq n$. Then the path $P'$ formed by appending $\ell$ copies of $\Gamma^*$ to the end of $P$ is also a shortest $s$-$v$ path. Hence, the subpath $P''$ of $P'$ formed by the first $n$ edges of $P'$, which is an $s$-$v^*$ path for some $v^* \in V$, is a shortest $s$-$v^*$ path. Therefore, $d_n'(v^*) = c'(P'') = \min_{0 \leq k \leq n - 1} d_k'(v^*)$. This proves that
$$ \min_{j \in V} \max_{0 \leq k \leq n - 1} \frac{d_n'(j) - d_k'(j)}{n - k} = 0. $$
Let $j \in V$. Let $0 \leq k \leq n$. Let $P$ be a shortest $s$-$j$ path of length $k$. Then $d_k(j) = c(P)$. It is clear that $P$ is also a shortest $s$-$j$ path of length $k$ with edge costs $c'$. Hence, $d_k'(j) = c'(P)$. Since $d_k(j)$ is a path of length $k$, then we have that
\begin{align*}
  d_k(j) &= c(P) = \sum_{e \in E(P)} c(e) = \sum_{e \in E(P)} (c(e) - \mu + \mu) = \sum_{e \in E(P)} (c(e) - \mu) + |P| \mu \\
  &= \sum_{e \in E(P)} c'(e) + k \mu = c'(P) + k\mu = d_k'(j) + k\mu.
\end{align*}
Hence, we have that
\begin{align*}
  \min_{j \in V} \max_{0 \leq k \leq n - 1} \frac{d_n(j) - d_k(j)}{n - k} &= \min_{j \in V} \max_{0 \leq k \leq n - 1} \frac{\left(d_n'(j) + n\mu\right) - \left(d_k'(j) + k\mu\right)}{n - k} \\
  &= \min_{j \in V} \max_{0 \leq k \leq n - 1} \frac{d_n'(j) - d_k'(j) + (n - k) \mu}{n - k} \\
  &= \min_{j \in V} \max_{0 \leq k \leq n - 1} \left(\frac{d_n'(j) - d_k'(j)}{n - k} + \mu\right) \\
  &= \min_{j \in V} \max_{0 \leq k \leq n - 1} \frac{d_n'(j) - d_k'(j)}{n - k} + \mu \\
  &= 0 + \mu = \mu.
\end{align*}

Next, we show that $d_k(j)$ can be computed by the following recurrence:
\begin{equation} \label{eq:bellman-ford-recurrence}
  d_k(j) = \left\{
  \begin{array}{ll}
    \min_{(i, j) \in E} \left(d_{k - 1}(i) + c(i, j)\right), & k > 0, \\
    0, & k = 0, j = s, \\
    \infty, & k = 0, j \neq s.
  \end{array}
\right.
\end{equation}
It is clear that $d_0(s) = 0$ and $d_0(j) = \infty$ for all $j \in V \setminus \{ s \}$. Let $1 \leq k \leq n$. Let $j \in V$. Let $P$ be a shortest $s$-$j$ path of length $k$. Let $(i^*, j)$ be the last edge of $P$. Then the subpath $P'$ formed by all edges of $P$ except $(i^*, j)$ is a shortest $s$-$i^*$ path of length $k - 1$. Hence, $c(P') = d_{k - 1}(i^*)$. This implies that
$$ d_k(j) = c(P) = c(P') + c(i^*, j) = d_{k - 1}(i^*) + c(i^*, j) \geq \min_{(i, j) \in E} \left(d_{k - 1}(i) + c(i, j)\right). $$
For all $(i, j) \in E$, if $P_i$ is a shortest $s$-$i$ path of length $k - 1$, then $P_i$ appended by $(i, j)$ is an $s$-$j$ path, so $d_{k - 1}(i) + c(i, j) = c(P_i) + c(i, j) \geq d_k(j)$. This implies that $\min_{(i, j) \in E} (d_{k - 1}(i) + c(i, j)) \geq d_k(j)$. This proves \eqref{eq:bellman-ford-recurrence}. We give Algorithm \ref{alg:min-mean-cost-cycle} to compute $\mu$ and a cycle $\Gamma$ such that $\mu = \frac{c(\Gamma)}{|\Gamma|}$. It is clear that the running time of Algorithm \ref{alg:min-mean-cost-cycle} is $O(nm)$. It remains to show that $\Gamma^*$ returned by Algorithm \ref{alg:min-mean-cost-cycle} satisfies $\frac{c(\Gamma^*)}{|\Gamma^*|} = \mu$. We note that $p_k(j)$ stores a shortest $s$-$j$ path of length $k$ by following $p_k(j)$ backwards. Hence, $P$ is a shortest $s$-$j^*$ path of length $n$. This implies that $P$ is not simple and hence contains at least one cycle. Since $\frac{d_n(j^*) - d_{k^*}(j^*)}{n - k^*} = \mu$, then we have that
\begin{align*}
  \frac{d_n'\left(j^*\right) - d_{k^*}'\left(j^*\right)}{n - k^*} &= \frac{\left(d_n\left(j^*\right) - n\mu\right)- \left(d_{k^*}\left(j^*\right) - k^* \mu\right)}{n - k^*} = \frac{d_n\left(j^*\right) - d_{k^*}\left(j^*\right) - \left(n - k^*\right) \mu}{n - k^*} \\
  &= \frac{d_n\left(j^*\right) - d_{k^*}\left(j^*\right)}{n - k^*} - \mu = \mu - \mu = 0.
\end{align*}
This implies that $d_n'(j^*) = d_{k^*}'(j^*) = \min_{0 \leq k \leq n - 1} d_k'(j^*)$ is the length of the shortest $s$-$j^*$ path. Hence, cycle $\Gamma^*$ contained in $P$ must have cost $0$ with edge costs $c'$. Otherwise, we could have eliminated $\Gamma^*$ to get a lower cost. We have that
\begin{align*}
  \frac{c\left(\Gamma^*\right)}{\left|\Gamma^*\right|} &= \frac{\sum_{e \in E\left(\Gamma^*\right)} c(e)}{\left|\Gamma^*\right|} = \frac{\sum_{e \in E\left(\Gamma^*\right)} (c(e) - \mu + \mu)}{\left|\Gamma^*\right|} = \frac{\sum_{e \in E\left(\Gamma^*\right)} (c(e) - \mu) + \left|\Gamma^*\right| \mu}{\left|\Gamma^*\right|} \\
  &= \frac{\sum_{e \in E\left(\Gamma^*\right)} c'(e)}{\left|\Gamma^*\right|} + \mu = \frac{c'\left(\Gamma^*\right)}{\left|\Gamma^*\right|} + \mu = \frac{0}{\left|\Gamma^*\right|} + \mu = 0 + \mu = \mu.
\end{align*}
This completes the proof.

\begin{algorithm}
  $d_k(j) \leftarrow \infty$ for all $0 \leq k \leq n, j \in V$ \\
  $d_0(s) \leftarrow 0$ \\
  $p_k(j) \leftarrow \textbf{null}$ for all $0 \leq k \leq n, j \in V$ \\
  \For{$k \leftarrow 1, \ldots, n$}{
    \For{$(i, j) \in E$}{
      \If{$d_{k - 1}(i) + c(i, j) < d_k(j)$}{
        $d_k(j) \leftarrow d_{k - 1}(i) + c(i, j)$ \\
        $p_k(j) \leftarrow i$
      }
    }
  }
  $\mu \leftarrow \infty$ \\
  \For{$j \in V$}{
    $\nu \leftarrow -\infty$ \\
    \For{$k \leftarrow 0, \ldots, n - 1$}{
      $\nu \leftarrow \max(\nu, \frac{d_n(j) - d_k(j)}{n - j})$
    }
    \If{$\nu < \mu$}
    {
      $\mu \leftarrow \nu$ \\
      $j^* \leftarrow j$
    }
  }
  $P = \{ (v_1, v_2), \ldots, (v_{n - 1}, v_n) \} \leftarrow \text{path formed by following $p_n$ from $j^*$ backwards}$ \\
  \For{$p \leftarrow 1, \ldots, n - 1$}{
    \For{$q \leftarrow p + 1, \ldots, n$}{
      \If{$v_p = v_q$}{
        \Return{$\Gamma^* = \{ (v_p, v_{p + 1}), \ldots, (v_{q - 1}, v_q) \}$}
      }
    }
  }
  \caption{An algorithm for computing the minimum mean-cost cycle.}
  \label{alg:min-mean-cost-cycle}
\end{algorithm}

\bibliographystyle{abbrvnat}
\bibliography{bellmanford.bib}

\end{document}
